Allow environment weakening to reorder declarations
This is a significant reorganization of the handling of declaration
extension, with the goal of allowing environment weakening across
reordering of independent declarations.  This will be useful for using
the safechecker to concretely prove different constructions well-typed
in minimal global environments, and then combine the well-typedness
proofs in a union of the global environments without having to care
about strict extension.

We define four notions of environment extension.  The two configurable
bits are: is universe and retroknowledge extension strict (`Logic.eq`)
or loose (`⊂_cs` / `Retroknowledge.extends`); and is declaration
extension strict (fully order-preserving, i.e., new declarations are
added only at the front) or lax (declarations may be reordered and added
freely, as long as all new declarations with existing names come before
the old ones with the same names, and the relative order of declarations
with identical names is preserved).

In most cases, we are actually interested only in duplicate-free
environments, where the lax construction is equivalent to merely
requiring that the lookup function agrees on all existing delcarations.
However, we formulate the property in a way that makes sense for
duplicative environments so that strict declaration extension will
always imply lax declaration extension.  (The lookup function prefers
earlier / newer declarations over older ones.)

We thus have the following implication structure:
```
┌-----------------------------┬------------------------┬---------------------------┐
|    univ/retro extension is: |        strict          |  lax                      |
├ declaration exension is ----┼------------------------┼---------------------------┤
|    lax                      |     extends_decls      →         extends           |
|                             |            ↑           ↗            ↑              |
|   strict                    | strictly_extends_decls → extends_strictly_on_decls |
└-----------------------------┴------------------------┴---------------------------┘
```

In general, theorems use the strictest version permissible in the
conclusion (more generally in covariant positions), and the laxest
version permissible in their hypotheses (more generally in contravariant
positions).  Some theorems are parameterized over their notion of
context extension, when the version in the conclusion and the hypotheses
(more generally: isovariant positions) must match.

The exception to this rule is `SingletonProp`, `Computational`,
`Informative`, `erases`, and their dependents.  These definitions and
theorems uniformly use `strictly_extends_decls`, because I wasn't sure
if it was worth the effort to generalize these definitions over their
notion of extension, and the definitions seem to be used in both co- and
contra-variant positions.

template-coq/theories/Environment.v
@@ -361,18 +361,71 @@ Module Environment (T : Term).
 
   Definition lookup_env (Σ : global_env) (kn : kername) := lookup_global Σ.(declarations) kn.
 
+  (* version for possibly duplicative environments *)
+  Fixpoint lookup_globals (Σ : global_declarations) (kn : kername) : list global_decl :=
+    match Σ with
+    | nil => nil
+    | d :: tl =>
+        let tl := lookup_globals tl kn in
+        if kn == d.1 then d.2 :: tl else tl
+    end.
+
+  Definition lookup_envs (Σ : global_env) (kn : kername) := lookup_globals Σ.(declarations) kn.
+
+  (** We define four notions of environment extension.  The two
+      configurable bits are: is universe and retroknowledge extension
+      strict ([Logic.eq]) or loose ([⊂_cs] / [Retroknowledge.extends]);
+      and is declaration extension strict (fully order-preserving,
+      i.e., new declarations are added only at the front) or lax
+      (declarations may be reordered and added freely, as long as all
+      new declarations with existing names come before the old ones
+      with the same names, and the relative order of declarations with
+      identical names is preserved).
+
+      In most cases, we are actually interested only in duplicate-free
+      environments, where the lax construction is equivalent to merely
+      requiring that the lookup function agrees on all existing
+      delcarations.  However, we formulate the property in a way that
+      makes sense for duplicative environments so that strict
+      declaration extension will always imply lax declaration
+      extension.  (The lookup function prefers earlier / newer
+      declarations over older ones.)
+
+      We thus have the following implication structure:
+<<<
+┌-----------------------------┬------------------------┬---------------------------┐
+|    univ/retro extension is: |        strict          |  lax                      |
+├ declaration exension is ----┼------------------------┼---------------------------┤
+|    lax                      |     extends_decls      →         extends           |
+|                             |            ↑           ↗            ↑              |
+|   strict                    | strictly_extends_decls → extends_strictly_on_decls |
+└-----------------------------┴------------------------┴---------------------------┘
+>>>
+   *)
   Definition extends (Σ Σ' : global_env) :=
     [× Σ.(universes) ⊂_cs Σ'.(universes),
-      ∑ Σ'', Σ'.(declarations) = Σ'' ++ Σ.(declarations) &
+      forall c, ∑ decls, lookup_envs Σ' c = decls ++ lookup_envs Σ c &
       Retroknowledge.extends Σ.(retroknowledge) Σ'.(retroknowledge)].
 
   Definition extends_decls (Σ Σ' : global_env) :=
     [× Σ.(universes) = Σ'.(universes),
-       ∑ Σ'', Σ'.(declarations) = Σ'' ++ Σ.(declarations) &
-       Σ.(retroknowledge) = Σ'.(retroknowledge)].
+      forall c, ∑ decls, lookup_envs Σ' c = decls ++ lookup_envs Σ c &
+      Σ.(retroknowledge) = Σ'.(retroknowledge)].
+
+  Definition extends_strictly_on_decls (Σ Σ' : global_env) :=
+    [× Σ.(universes) ⊂_cs Σ'.(universes),
+      ∑ Σ'', Σ'.(declarations) = Σ'' ++ Σ.(declarations) &
+      Retroknowledge.extends Σ.(retroknowledge) Σ'.(retroknowledge)].
+
+  Definition strictly_extends_decls (Σ Σ' : global_env) :=
+    [× Σ.(universes) = Σ'.(universes),
+      ∑ Σ'', Σ'.(declarations) = Σ'' ++ Σ.(declarations) &
+      Σ.(retroknowledge) = Σ'.(retroknowledge)].
 
   Existing Class extends.
   Existing Class extends_decls.
+  Existing Class extends_strictly_on_decls.
+  Existing Class strictly_extends_decls.
 
   Lemma lookup_global_None Σ kn : ~In kn (List.map fst Σ) <-> lookup_global Σ kn = None.
   Proof.
@@ -380,17 +433,89 @@ Module Environment (T : Term).
     move => ??; case: eqb_spec; intuition congruence.
   Qed.
 
+  Lemma hd_error_lookup_globals Σ kn : hd_error (lookup_globals Σ kn) = lookup_global Σ kn.
+  Proof.
+    move: Σ; elim => //= ?? <-.
+    case: eqb_spec => //=.
+  Qed.
+
+  Lemma lookup_globals_nil Σ kn : ~In kn (List.map fst Σ) <-> lookup_globals Σ kn = nil.
+  Proof.
+    rewrite lookup_global_None-hd_error_lookup_globals.
+    case: lookup_globals => //.
+  Qed.
+
+  Lemma NoDup_length_lookup_globals Σ
+    : NoDup (List.map fst Σ)
+      -> forall kn, List.length (lookup_globals Σ kn) = match lookup_global Σ kn with
+                                                        | Some _ => 1
+                                                        | None => 0
+                                                        end.
+  Proof.
+    move => H kn.
+    move: Σ H; elim => //=; try lia.
+    move => ?? H. inversion 1; subst.
+    move: (H ltac:(assumption)).
+    case: eqb_spec => //= ->.
+    rewrite (proj1 (@lookup_global_None _ _)) => //= -> //=.
+  Qed.
+
+  Lemma lookup_globals_In Σ kn decl
+    : In (kn, decl) Σ <-> In decl (lookup_globals Σ kn).
+  Proof.
+    move: Σ; elim => //=; try tauto.
+    move => [??]?; case: eqb_spec => ? //=; subst => <-; cbn in *; firstorder (subst; auto).
+    all: (idtac + constructor); congruence.
+  Qed.
+
   Lemma lookup_global_Some_iff_In_NoDup Σ kn decl (H : NoDup (List.map fst Σ))
     : In (kn, decl) Σ <-> lookup_global Σ kn = Some decl.
   Proof.
-    move: Σ H; elim => //=; try tauto.
-    move => [??]?; case: eqb_spec => ? IH; inversion 1; subst; try rewrite <- IH by assumption.
-    all: intuition try congruence; subst.
-    all: cbn in *.
-    all: repeat match goal with H : (_, _) = (_, _) |- _ => inversion H; clear H end.
-    all: repeat match goal with H : Some _ = Some _ |- _ => inversion H; clear H end.
-    all: subst => //=; auto.
-    all: try now epose proof (@in_map _ _ fst _ (_, _)); cbn in *; exfalso; eauto.
+    rewrite -hd_error_lookup_globals lookup_globals_In.
+    apply NoDup_length_lookup_globals with (kn:=kn) in H; move: H.
+    case: lookup_global; case: lookup_globals => [|?[]]; cbn.
+    all: try lia.
+    all: intuition congruence.
+  Qed.
+
+  Lemma lookup_env_extends_NoDup Σ Σ' k d :
+    NoDup (List.map fst Σ'.(declarations)) ->
+    lookup_env Σ k = Some d ->
+    extends Σ Σ' -> lookup_env Σ' k = Some d.
+  Proof.
+    rewrite /lookup_env /= -!hd_error_lookup_globals => Hnd.
+    move: (@NoDup_length_lookup_globals _ Hnd k); clear Hnd.
+    rewrite -hd_error_lookup_globals.
+    move=> H Hd [? eq].
+    move: (eq k); clear eq.
+    rewrite /lookup_envs.
+    case => ls eq.
+    move: eq Hd H => ->.
+    case: ls => //= ?.
+    case => //=.
+    case: lookup_globals => //=.
+  Qed.
+
+  Lemma lookup_globals_app Σ Σ' kn :
+    lookup_globals (Σ ++ Σ') kn = lookup_globals Σ kn ++ lookup_globals Σ' kn.
+  Proof.
+    move: Σ.
+    elim => //= ??.
+    case: eqb_spec => //= -> -> //=.
+  Qed.
+
+  #[global] Instance strictly_extends_decls_extends_decls Σ Σ' : strictly_extends_decls Σ Σ' -> extends_decls Σ Σ'.
+  Proof.
+    destruct Σ, Σ'; case => //= -> [Σ'' ->] ->.
+    rewrite /extends_decls/lookup_envs //=; split => //= ?.
+    rewrite lookup_globals_app.
+    eexists; reflexivity.
+  Qed.
+
+  #[global] Instance strictly_extends_decls_extends_strictly_on_decls Σ Σ' : strictly_extends_decls Σ Σ' -> extends_strictly_on_decls Σ Σ'.
+  Proof.
+    destruct Σ, Σ'; intros []. cbn in *; subst. split => //=.
+    split; [lsets|csets]. apply Retroknowledge.extends_refl.
   Qed.
 
   #[global] Instance extends_decls_extends Σ Σ' : extends_decls Σ Σ' -> extends Σ Σ'.
@@ -399,11 +524,31 @@ Module Environment (T : Term).
     split; [lsets|csets]. apply Retroknowledge.extends_refl.
   Qed.
 
+  #[global] Instance extends_strictly_on_decls_extends Σ Σ' : extends_strictly_on_decls Σ Σ' -> extends Σ Σ'.
+  Proof.
+    destruct Σ, Σ'; case => //= ? [Σ'' ->] ?.
+    rewrite /extends/lookup_envs //=; split => //= ?.
+    rewrite lookup_globals_app.
+    eexists; reflexivity.
+  Qed.
+
+  #[global] Instance strictly_extends_decls_extends_decls_subrel : CRelationClasses.subrelation strictly_extends_decls extends_decls := strictly_extends_decls_extends_decls.
+  #[global] Instance strictly_extends_decls_extends_strictly_on_decls_subrel : CRelationClasses.subrelation strictly_extends_decls extends_strictly_on_decls := strictly_extends_decls_extends_strictly_on_decls.
+  #[global] Instance extends_decls_extends_subrel : CRelationClasses.subrelation extends_decls extends := extends_decls_extends.
+  #[global] Instance extends_strictly_on_decls_extends_subrel : CRelationClasses.subrelation extends_strictly_on_decls extends := extends_strictly_on_decls_extends.
+  #[global] Instance strictly_extends_decls_extends_subrel : CRelationClasses.subrelation strictly_extends_decls extends := fun _ => _.
+
+  #[global] Instance strictly_extends_decls_refl : CRelationClasses.Reflexive strictly_extends_decls.
+  Proof. red. intros x. split => //; try exists [] => //. Qed.
+
   #[global] Instance extends_decls_refl : CRelationClasses.Reflexive extends_decls.
   Proof. red. intros x. split => //; try exists [] => //. Qed.
 
+  Lemma extends_strictly_on_decls_refl : CRelationClasses.Reflexive extends_strictly_on_decls.
+  Proof. red. intros x. split; [apply incl_cs_refl | try exists [] => // | apply Retroknowledge.extends_refl]. Qed.
+
   Lemma extends_refl : CRelationClasses.Reflexive extends.
-  Proof. red. intros x. split; [apply incl_cs_refl | now exists [] | apply Retroknowledge.extends_refl]. Qed.
+  Proof. red. intros x. split; [apply incl_cs_refl | try exists [] => // | apply Retroknowledge.extends_refl]. Qed.
 
   (* easy prefers this to the local hypotheses, which is annoying
   #[global] Instance extends_refl : CRelationClasses.Reflexive extends.
@@ -422,7 +567,11 @@ Module Environment (T : Term).
                  | split
                  | intro
                  | now eexists; rewrite app_assoc ].
+  #[global] Instance strictly_extends_decls_trans : CRelationClasses.Transitive strictly_extends_decls.
+  Proof. extends_trans_t. Qed.
   #[global] Instance extends_decls_trans : CRelationClasses.Transitive extends_decls.
+  Proof. extends_trans_t. Qed.
+  #[global] Instance extends_strictly_on_decls_trans : CRelationClasses.Transitive extends_strictly_on_decls.
   Proof. extends_trans_t. Qed.
   #[global] Instance extends_trans : CRelationClasses.Transitive extends.
   Proof. extends_trans_t. Qed.
